values_are_integers done in Definability but to refactor since very brittle
There is a good amount of case analysis but chaining all of them in one
go wouldn't be very nice either. For now relying on goal selectors, but
would be refactored with Ltac for instance.

Re-introduced a variant of suffixes_of_seq with equivalence between the
two of them.

Common/Traces.v
@@ -40,20 +40,41 @@ Proof. by rewrite /suffix -lock /= orbF. Qed.
     (since we don't look at the events, we can use a sequence of type T)
  *)
 
-Definition suffixes_of_seq s : seq (seq T) :=
-  let fix aux s (acc:seq (seq T)) :=
-      match s with
-      | [::]  => acc
-      | h::t => aux t ((h::t)::acc)
-      end in
-  rev (aux s [::]).
+Let Fixpoint suffixes_of_seq_aux s acc :=
+  match s with
+  | [::]  => acc
+  | h::t => suffixes_of_seq_aux t ((h::t)::acc)
+  end.
+Definition suffixes_of_seq s := rev (suffixes_of_seq_aux s [::]).
 
 (* Non tail-recursive but still fairly efficient (doesn't use append) *)
-(* Fixpoint suffixes_of_seq' s : seq (seq T) := *)
-(*   match s with *)
-(*   | [::]  => [::] *)
-(*   | h::t => (h::t) :: suffixes_of_seq' t *)
-(*   end. *)
+Fixpoint suffixes_of_seq' s :=
+  match s with
+  | [::]  => [::]
+  | h::t => (h::t) :: suffixes_of_seq' t
+  end.
+
+Local Lemma suffixes_of_seq_aux_invar : forall s acc res,
+   suffixes_of_seq_aux s acc = res ->
+    exists res', suffixes_of_seq' s = res' /\
+            res = rev res' ++ acc.
+Proof.
+  induction s as [|h t IHt].
+  - by intros ; exists [].
+  - intros acc res H. apply IHt in H. destruct H as [res' [H1 H2]].
+    simpl. exists ((h::t)::res'). subst.
+    split ; first done ;
+      last by rewrite rev_cons -cat_rcons.
+Qed.
+
+Lemma suffixes_of_seq_equiv s : suffixes_of_seq s = suffixes_of_seq' s.
+Proof.
+  rewrite /suffixes_of_seq.
+  have H: suffixes_of_seq_aux s [] = suffixes_of_seq_aux s [] by [].
+  apply suffixes_of_seq_aux_invar in H.
+  destruct H as [ ? [? H]] ; subst. by rewrite H cats0 revK.
+Qed.
+
 
 Definition suffix_flip a b := suffix b a.
 
@@ -83,9 +104,6 @@ Proof. rewrite /subpred/suffix_flip. move => suffix. by apply suffix_prepended. 
 (*   all_sfxs t suffxs -> all_sfxs (x::t) suffxs. *)
 (* Proof. *)
 
-(* RB: STATIC_READ: Missing definition, used later and for now aliased to a
-   previous one. To fix. *)
-Definition suffixes_of_seq' := suffixes_of_seq.
 
 Lemma suffixes_of_seq_correct seq :
   all (suffix_flip seq) (suffixes_of_seq' seq) /\
